fstar/test/MLS.Test.FromExt.Welcome.fst
@@ -48,7 +48,8 @@ let test_welcome_one t =
 
     let kp_ref = extract_result (make_keypackage_ref #bytes (serialize _ key_package)) in
 
-    let (group_info, group_secrets, (_, my_init_decryption_key)) = extract_result (decrypt_welcome welcome (fun ref -> if ref = kp_ref then Some init_priv else None) (fun x -> return x)) in
+    let (group_secrets, (_, my_init_decryption_key)) = extract_result (decrypt_group_secrets welcome (fun ref -> if ref = kp_ref then Some init_priv else None) (fun x -> return x)) in
+    let group_info = extract_result (decrypt_group_info group_secrets.joiner_secret [] welcome.encrypted_group_info) in
 
     if not (verify_welcome_group_info signer_pub group_info) then (
       failwith "test_welcome_one: bad signature"
